thy/IP_Addresses/IPv4.thy
@@ -284,6 +284,6 @@ subsection\<open>IP Ranges: Examples\<close>
       let netmask = (mask len) << (32 - len);
           network_prefix = (pre AND netmask)
       in (network_prefix, network_prefix OR (NOT netmask)))"
-  by(simp add: ipcidr_to_interval_def Let_def ipcidr_to_interval_start.simps ipcidr_to_interval_end.simps)
+    by(simp add: ipcidr_to_interval_def Let_def ipcidr_to_interval_start.simps ipcidr_to_interval_end.simps)
  
 end
