thy/LOFT/Examples/SQRL/SQRL_Router.thy
@@ -1,0 +1,109 @@
+theory SQRL_Router
+  imports
+    "../../../Iptables_Semantics/Primitive_Matchers/Parser"
+    "../../../Routing/IpRoute_Parser"
+    "../../LinuxRouter_OpenFlow_Translation"
+    "../../OpenFlow_Serialize"
+begin
+  
+parse_iptables_save SQRL_fw="iptables-save"
+parse_ip_route SQRL_rtbl_main = "ip-route"
+definition "ipassmt \<equiv> let
+  a = ipv4addr_of_dotdecimal;
+  i = \<lambda>(b,c,d,e,f). ipcidr_tuple_to_wordinterval (a (b,c,d,e), f);
+  m = \<lambda>(i,b,c,d,e,f::nat). (Iface i, [(a (b,c,d,e), f)])
+  in [
+  m (''ldit'', 10,13,42,136,29),
+  m (''lmd'', 10,13,42,128,29),
+  m (''loben'', 10,13,42,144,28),
+  (Iface ''lup'', cidr_split (wordinterval_setminus wordinterval_UNIV
+    (wordinterval_Union [i (192,168,0,0,16), i (10,0,0,0,8), i (127,16,0,0,12)]))),
+  m (''vocb'', 10,13,43,16,28),
+ (Iface ''vpriv'', [(a (10,13,44,0),24), (a (10,13,37,0),24)]),
+  m (''vshit'', 10,13,43,0,28),
+  m (''wg'', 10,13,41,0,27),
+  m (''wt'', 10,13,42,160,28)
+] :: (iface \<times> (32 word \<times> nat) list) list"
+
+term SQRL_fw
+thm SQRL_fw_def
+thm SQRL_fw_FORWARD_default_policy_def
+value ipassmt
+find_theorems odd
+typ "32 word"
+
+value[code] "map (\<lambda>(c,rs). (c, map (quote_rewrite \<circ> common_primitive_rule_toString) rs)) SQRL_fw"
+definition "unfolded = unfold_ruleset_FORWARD SQRL_fw_FORWARD_default_policy (map_of_string_ipv4 SQRL_fw)"
+definition "sanitized assmt rtblo \<equiv> 
+  (upper_closure (optimize_matches abstract_for_simple_firewall (*(abstract_primitive 
+    (\<lambda>r. case r of Pos a \<Rightarrow> is_L4_Flags a | Neg a \<Rightarrow> is_L4_Flags a))*)
+  (upper_closure (iface_try_rewrite assmt rtblo
+  (upper_closure (packet_assume_new unfolded))))))"
+
+lemma "length unfolded = 69" by eval
+
+value[code] "unfolded"
+value[code] "(upper_closure unfolded)"
+value[code] "map (quote_rewrite \<circ> common_primitive_rule_toString) (upper_closure unfolded)"
+lemma "length (upper_closure unfolded) = 69" by eval
+
+
+value[code] "upper_closure (packet_assume_new unfolded)"
+  
+lemma "length (lower_closure unfolded) = 55" by eval
+
+(* say we'd happen to forget to abstract for simple_fw / remove the l4 matches *)
+value[code] "report_simple_fw_preconditions (upper_closure (packet_assume_new unfolded))"
+
+lemma "check_simple_fw_preconditions (sanitized ipassmt None)" by eval
+lemma "check_simple_fw_preconditions (sanitized ipassmt (Some SQRL_rtbl_main))" by eval
+    
+(* quick look at the access matrix (for http): *)
+value[code] "let m = access_matrix_pretty_ipv4 parts_connection_http
+  (to_simple_firewall_without_interfaces ipassmt (Some SQRL_rtbl_main) 
+    unfolded);
+  f = the \<circ> map_of (fst m) in
+  map (map_prod f f) (snd m)"
+(* but that's not what we're here for. *)
+
+  
+
+definition "SQRL_fw_simple \<equiv> remdups_rev (to_simple_firewall (sanitized ipassmt (Some SQRL_rtbl_main)))"
+lemma "simple_fw_valid SQRL_fw_simple" by eval
+lemma "length SQRL_fw_simple = 618" by eval
+value[code] "SQRL_fw_simple"
+lemma "simple_fw_valid SQRL_fw_simple" by eval
+(* fun fact: *)
+lemma "no_oif_match SQRL_fw_simple" by eval
+(* I mean, we can abstract over interfaces using
+  upper_closure \<circ> optimize_matches (abstract_primitive
+  (\<lambda>r. case r of Pos a \<Rightarrow> is_Oiface a | Neg a \<Rightarrow> is_Oiface a))
+  The fun part is that we don't have to do that. *)
+
+definition "SQRL_ports \<equiv> [
+  (''ldit'', ''1''),
+  (''lmd'', ''2''),
+  (''loben'', ''3''),
+  (''lup'', ''4''),
+  (''vocb'', ''5''),
+  (''vpriv'', ''6''),
+  (''vshit'', ''7''),
+  (''wg'', ''8''),
+  (''wt'', ''9'')
+]"
+
+definition "ofi \<equiv> 
+    case (lr_of_tran SQRL_rtbl_main SQRL_fw_simple (map fst SQRL_ports))
+    of (Inr openflow_rules) \<Rightarrow> map (serialize_of_entry (the \<circ> map_of SQRL_ports)) openflow_rules"
+lemma "length ofi = 606" by eval
+value[code] ofi
+
+(* TODO: Well, that's something\<dots> I'd really like to have a proper file with newlines though\<dots> *)
+(*ML\<open>
+	val evterm = the (Code_Evaluation.dynamic_value @{context} @{term "intersperse (Char Nibble0 NibbleA) ofi"});
+	val opstr = Syntax.string_of_term (Config.put show_markup false @{context}) evterm;
+	File.write (Path.explode (File.platform_path(Resources.master_directory @{theory}) ^ "/pretty_str.txt")) opstr;
+\<close>*)
+
+end
+  
